```java
public static void main(String[] args) {
	int w = f(2,3);
}

static int f(int z, int x) {
	System.out.println(z + " " + x);
	if (z == x) {
		return 1;
	}
	if (z ==0) {
		return 1;
	}
	return f(z, x-1) + f(z-1, x-1);
}
```

```java
int w = f(2, 3) = 3
    > 2 3
    f(2, 3-1) 1 = 2
        > 2 2
        return 1
     f(2-1, 3-1) = 1 + 1
         > 1 2
         f(1, 2-1) = 1
             > 1 1
             return 1
         f(1-1, 2-1) = 1
             > 0 1
             return 1

> 2 3
> 2 2
> 1 2
> 1 1
> 0 1
```
